$S=\left\{\vec u_1,\vec u_2,\dots,\vec u_n\right\}$ to $S'=\left\{\vec v_1,\vec v_2,\dots,\vec v_n\right\}$ 
$$\begin{aligned}
\vec v_1 &= a_{11}\vec u_1 + a_{12}\vec u_2 + \cdots + a_{1n}\vec u_n\\
\vec v_2 &= a_{21}\vec u_1 + a_{22}\vec u_2 + \cdots + a_{2n}\vec u_n\\
\cdots&\cdots\cdots\cdots\cdots\cdots\cdots\cdots\cdots\cdots\cdots \\
\vec v_n &= a_{n1}\vec u_1 + a_{n2}\vec u_2 + \cdots + a_{nn}\vec u_n\\
\end{aligned}$$
$P$ the matrix transpose of above matrix of coefficients is called change of basis matrix.
- $$P=\left[[v_1]_S,[v_2]_S,\dots,[v_n]_S\right]$$
- $$P[v]_{S'}=[v]_S$$